\hypertarget{haskell-lists-and-patterns}{%
\subsection{Haskell Lists and Patterns}\label{haskell-lists-and-patterns}}

\hypertarget{list-sugaring}{%
\subsubsection{List sugaring}\label{list-sugaring}}

Rewrite the following expressions so that they don't contain the list
constructor : (`cons') any longer.

\begin{lstlisting}[language=Haskell]
s1 = 1 : 2 : 3 : [4] = [1,2,3,4]
s2 = 1 : 2 : [3 , 4] = [1,2,3,4]
s3 = (1 : 2 : []) : (3 : []) : [[1,2],[3]]
s4 = (1 , 2) : (3 , 4) : [(5 , 6)] = [(1,2),(3,4),(5,6)]
s5 = [] : [] = [[]]
s6 = [] : [] : [] [[], []]
s7 = ([] : []) : [] = [[[]]]
s8 = (([] : []) : []) : [] = [[[[]]]]
s9 = 'a' : 'b' : [] = [ab] = "ab"
\end{lstlisting}

\hypertarget{list-desugaring}{%
\subsubsection{List desugaring}\label{list-desugaring}}

Rewrite the following expressions so that they contain the square
brackets {[}and{]} only as list constructor {[}{]} (`nil').

\begin{lstlisting}[language=Haskell]
d1 = [1 , 2 , 3] = 1 : 2 : 3 : []
d2 = [[1 , 2] , [] , [3 , 4]] = (1 : [2]) : ([]) : (3 : [4]) : []
\end{lstlisting}

\hypertarget{pattern-matching}{%
\subsubsection{Pattern Matching}\label{pattern-matching}}

Given are the following function and value declarations. Give the type
of each function and evaluate the expressions in the value declarations.
Give reasons for possible errors in types or pattern matching.

\begin{lstlisting}[language=Haskell]
f1 (x: y: z) = (x, y, z)
f2 [x, y] = (x, y)
f3 (x : y : []) = (x, y)

a11 = f1 [] ==> error
a21 = f2 [] ==> error
a31 = f3 [] ==> error

a12 = f1 [1] ==> error
a22 = f2 [1] ==> error
a32 = f3 [1] ==> error

a13 = f1 [1,2] ==> (1,2,[]) :: Num b => (b, b, [b])
a23 = f2 [1,2] ==> (1,2) :: Num b => (b, b)
a33 = f3 [1,2] ==> (1,2) :: Num b => (b, b)

a14 = f1 [1, 2, 3] ==> (1,2,[3]) :: Num b => (b, b, [b])
a24 = f2 [1, 2, 3] ==> error
a34 = f3 [1, 2, 3] ==> error

a15 = f1 (1: 2: 3 :[]) ==> (1,2,[3]) :: Num b => (b, b, [b])
a25 = f2 (1: 2: 3 :[]) ==> error
a35 = f3 (1: 2: 3 :[]) ==> error

a16 = f1 ['a', 'b', 'c'] ==> ('a','b',"c") :: (Char, Char, [Char])
a17 = f1 [[1], [2,3], []] ==> ([1],[2,3],[[]]) :: Num a => ([a], [a], [[a]])
a18 = f1 (1: 2: 3: [4 ,5]) ==> (1,2,[3,4,5]) :: Num b => (b, b, [b])
a19 = f1 [1..100] ==> (1,2,[3,4,5,...,100]) :: (Num b, Enum b) => (b, b, [b])

g1 "dimdi " = 1
g1 ['d', 'o', 'm', 'd', 'o'] = 2
g1 ('d': 'i': 'n': 'g': []) = 3
g1 ('d': 'i': 'n': 'g': _) = 4
g1 (x : y) = 5
g1 _ = 6

b11 = g1 "domdo" ==> 2 :: Num p => p
b12 = g1 "ding" ==> 3 :: Num p => p
b13 = g1 "dingdimdi" ==> 4 :: Num p => p
b14 = g1 "dumdu" ==> 5 :: Num p => p  (x fuer den ersten Char, y fuer den Rest)
b15 = g1 "" ==> 6 :: Num p => p
\end{lstlisting}
